term.fst is completed, makefile modified, subst is incomplete

subst.fst
@@ -1,11 +1,87 @@
 module Subst
 
+open Term
+
 type subst = list (variable * term)
 
-val apply : subst -> term -> term
+val isnt_cyclic : subst -> Tot bool
+val get_term_list : subst -> Tot (list term)
+val get_var_list : subst -> Tot (list variable)
+val check_presence_varlist_termlist : list variable -> list term -> Tot bool
 
-val compose : subst -> subst -> subst
+val mem: #a:eqtype -> a -> list a -> Tot bool
+let rec mem #a x xs =
+  match xs with
+  | [] -> false
+  | hd::tl -> hd=x || mem x tl
 
+let rec get_term_list st =
+match st with
+| [] -> []
+| hd::tl -> (snd hd)::(get_term_list tl)
+
+let rec get_var_list st =
+match st with
+| [] -> []
+| hd::tl -> (fst hd)::(get_var_list tl)
+
+let rec check_presence_varlist_termlist lv lt =
+  match lv with
+  | [] -> true
+  | hd::tl -> (is_var_present_list hd lt) && (check_presence_varlist_termlist tl lt)
+
+let isnt_cyclic st =
+  let lv = get_var_list st in
+  let lt = get_term_list st in
+  check_presence_varlist_termlist lv lt
+
+
+val apply : subst -> term ->Tot term
+val apply_list : subst -> list term ->Tot (list term)
+
+val get_mem : variable -> subst -> Tot term
+
+
+(** bad function rewrite later**)
+let rec get_mem v st= match st with
+| hd::tl -> if (fst hd)=v then (snd hd) else (get_mem v tl)
+| [] -> Var v
+
+let rec apply st t =
+  match t with
+  | Var v -> if mem v (get_var_list st) then (get_mem v st) else t
+  | Func s args -> Func s (apply_list st args)
+  | Name n -> t
+  and apply_list st lt = match lt with
+  | [] -> []
+  | hd::tl -> (apply st hd)::(apply_list st tl)
+
+val compose : subst -> subst -> Tot subst
+
+let rec compose st1 st2 = match st1 with
+ | [] -> st2
+ | hd::tl -> hd::(compose tl st2)
+
+(*
 val is_unify : term -> term -> bool
 
-val mgs : t1:term -> t2:term{ is_unify t1 t2 } -> subst
+val mgs : t1:term -> t2:term{ is_unify t1 t2 } -> subst*)
+
+
+val ground_term_lemma : st:subst -> t:term -> Lemma (requires (is_ground t)) (ensures (apply st t)=t)
+
+let rec ground_term_lemma st t = match st with
+ | [] -> ()
+ | hd::tl -> ground_term_lemma tl t
+
+val compose_lemma : st1:subst -> st2:subst -> Lemma (requires true) (ensures (forall (t:term). apply (compose st1 st2) t = apply st2 (apply st1 t)))
+
+let rec compose_lemma st1 st2 = match st1 with
+ | [] -> ()
+ | hd::tl -> compose_lemma tl st2
+
+val assoc_lemma : st1:subst -> st2:subst -> Lemma (requires isnt_cyclic(compose st1 st2))(ensures forall (t:term). apply (compose st1 st2) t= apply st2 (apply st1 t) )
+
+let rec assoc_lemma st1 st2 = match st1 with
+| [] -> ()
+| hd::tl-> assoc_lemma tl st2
