term.fst
@@ -8,66 +8,124 @@ type symbol_cat =
   | Constructor: symbol_cat
   | Destructor: symbol_cat
 
-and symbol =
+type symbol =
   {
     name_s: string;
     arity: nat;
     category_s: symbol_cat
   }
 
-and quantifier =
+type quantifier =
   | Free
   | Existential
   | Universal
 
 
-and variable =
+type variable =
   {
     name: string;
     id: nat;
   }
 
-and name_cat =
+type name_cat =
   | Public
   | Private
 
-and name =
+type name =
   {
     name_n : string;
     id : nat
   }
 
-and term =
-  | Var : variable -> term
-  | Name : name -> term
+type term =
+  | Var : v:variable -> term
+  | Name : n:name -> term
   | Func : s:symbol -> l:(list term){ List.Tot.length l = s.arity } -> term
 
 (*** Testing functions ***)
+val is_variable : term ->Tot bool
+
+let is_variable t = Var? t
 
 val is_equal : term -> term -> Tot bool
+val is_equal_list : list term -> list term -> Tot bool
 
-val is_function : term -> bool
+let rec is_equal t1 t2 =
+  match t1,t2 with
+  | Var arg1 , Var arg2 -> (arg1=arg2)
+  | Name arg1 ,Name arg2 -> (arg1=arg2)
+  | Func s1 args1 ,Func s2 args2 -> (s1=s2)&&(is_equal_list args1 args2)
+  | _,_ -> false
+  and is_equal_list list1 list2 =
+  match list1,list2 with
+  | [],[] -> true
+  | hd1::tl1,hd2::tl2 -> (is_equal hd1 hd2)&&(is_equal_list tl1 tl2)
+  | _,_ -> false
+val is_function : term ->Tot  bool
 
-val is_name : term -> bool
+let is_function f = Func? f
 
-val is_variable : term -> bool
+val is_name : term ->Tot  bool
 
-val is_ground : term -> bool
+let is_name t = Name? t
+
+val is_ground : t:term ->Tot  bool
+val is_ground_list : list_term: list term ->Tot  bool
+
+let rec is_ground t =
+  match t with
+  | Var _ -> false
+  | Func _ args -> is_ground_list args
+  | _ -> true
+and is_ground_list list_term =
+match list_term with
+| [] -> true
+| hd::tl -> is_ground hd && is_ground_list tl
 
 val is_constructor : term -> bool
+
+let is_constructor t =
+  if not(is_function t) then false else
+  if Constructor? ((Func?.s t).category_s) then true else false
+
+
+val is_var_present : variable -> term -> Tot bool
+val is_var_present_list : variable -> list term -> Tot bool
+
+let rec is_var_present v t =
+  match t with
+  | Var x -> if x=v then true else false
+  | Name n -> false
+  | Func _ args -> is_var_present_list v args
+  and is_var_present_list v term_list =
+  match term_list with
+  | [] -> true
+  | hd::tl -> (is_var_present v hd) && (is_var_present_list v tl)
 
 (*** Generation function ****)
 
 val of_variable : variable -> term
 
+let of_variable v = Var v
+
 val of_name : name -> term
+
+let of_name n = Name n
 
 (*** Access function ****)
 
-val apply_function : symbol -> term list -> term
+val apply_function : s:symbol -> l:list term{ List.Tot.length l = s.arity }-> term
+
+let apply_function s l = Func s l
 
 val root : t:term{ is_function t } -> symbol
 
+let root t = Func?.s t
+
 val variable_of : t:term { is_variable t } -> variable
 
+let variable_of t = Var?.v t
+
 val name_of : t:term { is_name t } -> name
+
+let name_of t = Name?.n t
