Makefile
@@ -1,10 +1,16 @@
 FSTAR_LIB = FStar.Set.fst FStar.List.Tot.fst
 
-FILES = term.fst
+FILES = term.fst subst.fst
 FILES_INTERFACE = term_interface.fst subst_interface.fst
 
 all:
 	fstar.exe $(FSTAR_LIB) $(FILES)
 
+term:
+	fstar.exe $(FSTAR_LIB) term.fst
+
 interface:
 	fstar.exe $(FSTAR_LIB) $(FILES_INTERFACE)
+
+subst:
+	fstar.exe $(FSTAR_LIB) subst.fst
